TheoremsAboutAlgorithms/Partitions/Partition.lean
@@ -1,0 +1,162 @@
+import TheoremsAboutAlgorithms.Partitions.Cell
+import TheoremsAboutAlgorithms.Partitions.Defs
+import TheoremsAboutAlgorithms.Partitions.Fin
+import TheoremsAboutAlgorithms.Partitions.Split
+
+namespace Partition
+
+-- TODO: Why can't we use e.g. partition.insertLast' for partition : Partition n?
+def Partition (n : ℕ) := {split : Split n // split.IsPartition}
+
+-- TODO: Should we somehow incorporate the subtype definition here?
+def partitions (n : ℕ) : Set (Split n)
+  := {split | split.IsPartition}
+
+-- TODO: Improve this proof and add comments
+theorem partitions_0 : partitions 0 = {∅} := by
+  apply Set.eq_of_subset_of_subset
+  · intro split h
+    simp
+    have := eq_or_ne split ∅
+    cases this with
+      | inl h_eq => exact h_eq
+      | inr h_ne =>
+        have := Set.nonempty_iff_ne_empty.mpr h_ne
+        cases this with
+          | intro cell h_cell =>
+            have := eq_or_ne cell ∅
+            cases this with
+              | inl h_eq =>
+                cases h with
+                  | intro h_empty _ => rw [h_eq] at h_cell ; contradiction
+              | inr h_ne' =>
+                have := Set.nonempty_iff_ne_empty.mpr h_ne'
+                cases this with
+                  | intro fin _ => apply Fin.elim0 fin
+  · intro split h
+    simp at h
+    have h_empty_not_mem : ∅ ∉ split := by simp [h]
+    have h_cover : ∀ (x : Fin 0), ∃! (cell : Cell 0), ∃! (_ : cell ∈ split), x ∈ cell := by
+      intro x
+      apply Fin.elim0 x
+    exact And.intro h_empty_not_mem h_cover
+
+abbrev ℙ (n : ℕ) := partitions n
+
+def recursivePartitions (n : ℕ) : Set (Split n)
+  := match n with
+    | 0 => {∅}
+    | m + 1 => ⋃ partition ∈ ℙ m, partition.insertLast' (Nat.succ_pos m)
+
+abbrev ℙᵣ (n : ℕ) := recursivePartitions n
+
+-- TODO: Better name
+-- TODO: Provide the version for Split 0 as well
+theorem insertLast'_mem_mem_of_mem_of_last_not_mem
+    {n : ℕ}
+    {split : Split (n + 1)}
+    {split' : Split (n + 2)}
+    {cell : Cell (n + 1)}
+    {h_pos : n + 2 > 0}
+    (h_split : split' ∈ split.insertLast' h_pos)
+    (h_mem : cell ∈ split)
+    -- We need split : Split (n + 1) above so we can cast the Fin.last (otherwise we don't get n - 1 + 1 = n because
+    -- we don't have n ≥ 1).
+    -- TODO: This is wrong. Of course (Fin.last n) ∉ cell, because we only insert it via split.insertLastAt cell.
+    --       What we could to is take a cell' ∈ split' where (Fin.last n) ∉ cell' and show that cell'.castPred is in
+    --       split.
+    (h_last_not_mem : (Fin.last n) ∉ cell)
+  : cell.castSucc ∈ split' := by
+    simp [Split.insertLast', Split.insertLast] at h_split
+    cases h_split with
+      | intro targetCell h_targetCell =>
+        rw [← h_targetCell.right]
+        simp at *
+        sorry
+
+-- Here we show that if we take a partition of Fin n and apply the operation partition.insertLast', then every resulting
+-- split' is a partition of Fin (n + 1).
+-- TODO: What namespace should this reside in?
+theorem insertLast'_produces_partitions
+    -- We use split : Split (n + 1) here because that's the form we need it in further down below
+    {n : ℕ}
+    {partition : Split n}
+    {split : Split (n + 1)}
+    {h_pos : n + 1 > 0}
+    (h_partition : partition ∈ ℙ n)
+    (h_split : split ∈ partition.insertLast' h_pos)
+  : split.IsPartition := by
+    have h_empty_not_mem : ∅ ∉ split := by
+      simp [Split.insertLast', Split.insertLast] at h_split
+      cases h_split with
+        | intro cell h_cell =>
+          have h_empty_not_mem_split'
+            := Split.insertLastAt_empty_not_mem_of_empty_not_mem partition cell h_partition.left
+          rw [← h_cell.right]
+          exact (Split.cast_empty_not_mem_iff _ (partition.insertLastAt cell)).mpr h_empty_not_mem_split'
+    have h_cover : ∀ (x : Fin (n + 1)), ∃! (cell : Cell (n + 1)), ∃! (_ : cell ∈ split), x ∈ cell := by
+      intro x
+      have := eq_or_ne x (Fin.last n)
+      cases this with
+        | inl h_eq =>
+          -- TODO:
+          sorry
+        | inr h_ne =>
+          simp [Split.insertLast', Split.insertLast] at h_split
+          have x' := Fin.castPred x h_ne
+          have := h_partition.right x'
+          cases this with
+            | intro cell h_cell =>
+              simp at h_cell
+              have cell' := Cell.castSucc cell
+              exists cell'
+              simp
+              -- TODO: We need to show that casting cell yields cell' and have covering of x' and uniqueness follow from
+              --       that.
+              constructor
+              · constructor
+                · sorry
+                · sorry
+              · sorry
+    exact And.intro h_empty_not_mem h_cover
+
+theorem partitions_subset_recursivePartitions (n : ℕ) : ℙ n ⊆ ℙᵣ n := by
+  intro split h
+  cases n with
+    | zero => simp [partitions_0] at h ; exact h
+    | succ m =>
+      have : ∃! (cell : Cell (m + 1)), ∃! (h_cell : cell ∈ split), (Fin.ofNat m + 1) ∈ cell := by
+        cases h with
+          | intro _ h_cover => exact h_cover (Fin.ofNat m + 1)
+      cases this with
+        | intro cell h_cell_unique =>
+          -- TODO: Plan:
+          --        1. Take the split p' that results from removing the cell containing Fin.last m + 1 from split.
+          --        2. Show that this split is a partition of m.
+          --        3. Show that we get p from p' via the recursive construction.
+          sorry
+
+-- Maybe we can use Set.rangeSplitting here? It's noncomputable though.
+theorem recursivePartitions_subset_partitions (n : ℕ) : ℙᵣ n ⊆ ℙ n := by
+  intro split h
+  cases n with
+    | zero => simp [partitions_0, recursivePartitions] at * ; exact h
+    | succ m =>
+      -- TODO: Can we use something like Set.mem_range for this?
+      cases h with
+        | intro partitions h_partitions =>
+          simp at h_partitions
+          cases h_partitions.left with
+            | intro partition h_partition =>
+              -- TODO: Rewrite so it reads nicer
+              have := h_partitions.right
+              rw [← h_partition] at this
+              simp [Set.mem_iUnion] at this
+              exact insertLast'_produces_partitions this.left this.right
+
+theorem partitions_eq_recursivePartitions (n : ℕ) : ℙ n = ℙᵣ n := by
+  apply Set.eq_of_subset_of_subset
+  · exact partitions_subset_recursivePartitions n
+  · exact recursivePartitions_subset_partitions n
+
+end Partition
