TheoremsAboutAlgorithms/Partitions/Split.lean
@@ -1,0 +1,126 @@
+import Mathlib.Data.Setoid.Partition
+import TheoremsAboutAlgorithms.Partitions.Defs
+import TheoremsAboutAlgorithms.Partitions.Cell
+
+namespace Split
+
+def cast {n m : ℕ} (h : n = m) (split : Split n) : Split m
+  := Cell.cast h '' split
+
+theorem cast_empty_not_mem_iff {n m : ℕ} (h : n = m) (split : Split n)
+  : ∅ ∉ split.cast h ↔ ∅ ∉ split := by
+    constructor <;> intro _ _ <;> simp [cast, Cell.cast] at * <;> contradiction
+
+theorem cast_nonempty_iff {n m : ℕ} (h : n = m) (split : Split n)
+  : (split.cast h).Nonempty ↔ split.Nonempty := by simp [cast]
+
+def castSucc {n : ℕ} (split : Split n) : Split (n + 1)
+  := Cell.castSucc '' split
+
+-- TODO: Fix naming elem -> mem
+theorem castSucc_empty_elem_iff {n : ℕ} (split : Split n)
+  : ∅ ∈ split.castSucc ↔ ∅ ∈ split := by simp [castSucc, Cell.castSucc]
+
+def removeCell {n : ℕ} (split : Split n) (cell : Cell n) : Split n
+  := split \ singleton cell
+
+-- TODO: Maybe we can find a better name yet (it's alright, but not totally satisfactory).
+-- We don't require targetCell ∈ split, because we want to be able to have ∅ as a target cell as well.
+-- This is essentially split ↦ {targetCell.transform} ∪ (split \ {targetCell})
+def insertLastAt {n : ℕ} (split : Split n) (targetCell : Cell n) : Split (n + 1)
+  := (split.removeCell targetCell).castSucc.insert targetCell.insertLast
+
+theorem insertLastAt_castSucc_mem {n : ℕ} (split : Split n) (targetCell : Cell n)
+  : targetCell.castSucc ∈ split.insertLastAt targetCell := by
+    simp [insertLastAt, Cell.insertLast]
+    sorry
+
+theorem insertLastAt_Injective {n : ℕ} (split : Split n) : Function.Injective (split.insertLastAt) := by
+  intro x y h
+  --simp [insertLastAt] at h
+  have := (Set.ext_iff (s := split.insertLastAt x) (t := split.insertLastAt y)).mp h x.castSucc
+  --simp [insertLastAt] at *
+  sorry
+
+theorem insertLastAt_nonempty {n : ℕ} (split : Split n) (targetCell : Cell n)
+  : (split.insertLastAt targetCell).Nonempty
+    := Set.insert_nonempty _ _
+
+-- TODO: Can we simplify this proof?
+theorem insertLastAt_empty_not_mem_of_empty_not_mem
+  {n : ℕ} (split : Split n) (targetCell : Cell n) (h : ∅ ∉ split) : ∅ ∉ split.insertLastAt targetCell := by
+    simp [insertLastAt]
+    intro h_empty_elem
+    cases h_empty_elem with
+      | inl h_elem_insertLast =>
+        have := Cell.insertLast_nonempty targetCell
+        -- TODO: There has to be an easier way to show Set.Nonempty x → ∅ = x → False
+        rw [← h_elem_insertLast] at this
+        cases this with
+          | intro x h_x_elem_empty =>
+            have := Set.mem_empty_iff_false x
+            apply this.mp
+            exact h_x_elem_empty
+      | inr h_elem_removeCell =>
+        simp [removeCell] at h_elem_removeCell
+        have := Set.diff_subset split {targetCell}
+        have h_empty_not_mem_diff := Set.not_mem_subset this h
+        have h_empty_mem_diff := (castSucc_empty_elem_iff (split \ {targetCell})).mp h_elem_removeCell
+        contradiction
+
+theorem insertLastAt_is_disjoint_insert {n : ℕ} (split : Split n) (targetCell : Cell n)
+  : Disjoint {targetCell.insertLast} (split.removeCell targetCell).castSucc := by
+    apply disjoint_iff.mpr
+    simp [removeCell, castSucc, Fin.castSucc]
+    intro cell _ _
+    have h_k : ¬ (∀ (x : Fin (n + 1)), x ∈ cell.castSucc ↔ x ∈ targetCell.insertLast) := by
+      simp [not_iff]
+      exists (Fin.last n)
+      constructor
+      · intro
+        simp [Cell.insertLast]
+        exact Set.mem_insert _ _
+      · intro
+        apply Set.disjoint_singleton_left.mp
+        exact Cell.insertLast_is_disjoint_insert cell
+    have := Set.ext_iff (s := cell.castSucc) (t := targetCell.insertLast)
+    exact (not_congr this).mpr h_k
+
+-- TODO: Maybe we can find a better name yet (it's alright, but not totally satisfactory).
+-- TODO: Do we even need this if we have the version below?
+def insertLast {n : ℕ} (split : Split n) : Set (Split (n + 1))
+  := {split.insertLastAt cell | cell ∈ split.insert ∅}
+
+theorem insertLast_nonempty_of_mem
+  {n : ℕ}
+  {split : Split n}
+  {split' : Split (n + 1)}
+  (h : split' ∈ insertLast split)
+  : split'.Nonempty := by
+    simp [insertLast] at h
+    cases h with
+      | intro cell h_cell =>
+        rw [← h_cell.right]
+        exact insertLastAt_nonempty _ _
+
+def insertLast' {n : ℕ} (h : n > 0) (split : Split (n - 1)) : Set (Split n)
+  := cast (Nat.sub_add_cancel h) '' split.insertLast
+
+theorem insertLast'_nonempty_of_mem
+  {n : ℕ}
+  {h : n > 0}
+  {split : Split (n - 1)}
+  {split' : Split n}
+  (h : split' ∈ insertLast' h split)
+  : split'.Nonempty := by
+    simp [insertLast'] at h
+    cases h with
+      | intro split'' h_split'' =>
+        rw [← h_split''.right]
+        have h_split''_nonempty : split''.Nonempty := insertLast_nonempty_of_mem h_split''.left
+        simp [cast_nonempty_iff, h_split''_nonempty]
+
+def IsPartition {n : ℕ} (split : Split n) : Prop
+  := Setoid.IsPartition split
+
+end Split
